\question{
    [2-13] Define $IP:\ron\times\ron\to\rl$ by
    $IP(x,y)=\langle x,y\rangle$.
}
\begin{parts}
    \part{
        Find $D(IP)(a,b)$ and $(IP)'(a,b)$.
    }
    \begin{solution}
        Since inner product is a bilinear
        function, we have
        $$D(IP)(a,b)(x,y)=IP(a,y)+IP(x,b)
        =\langle a,y\rangle
        +\langle x,b\rangle.
        $$
        And since $\langle a,y\rangle
        +\langle x,b\rangle=
        a_1y_1+...+a_ny_n+b_1x_1+
        ...+b_nx_n$, we have
        $$(IP)'(a,b)=(b_1,...,b_n,
        a_1,...,a_n)=(b,a).$$
    \end{solution}
    \part{
        \label{2-13, b}
        If $f,g:\rl\to\ron$ are
        differentiable
        and $h:\rl\to\rl$ is defined by
        $h(t)=\langle f(t),g(t)\rangle$,
        show that
        $$h'(a)=\langle f'(a)^T,g(a)\rangle
        +\langle f(a),g'(a)^T\rangle.$$
    }
    \begin{solution}
        Here, we can write $h$ as
        $h=(IP)\circ(f, g)$. Then
        \begin{align*}
            h'(a)&= (IP)'(f(a),g(a))\cdot
            \left(\begin{matrix}
                f'(a)\\g'(a)
            \end{matrix}\right)\\
            &=(g(a),f(a))\cdot
            \left(\begin{matrix}
                f'(a)\\g'(a)
            \end{matrix}\right)\\
            &=\sum_{i=1}^n
            {g_i(a)\cdot f_i'(a)}+
            \sum_{i=1}^n
            {f_i(a)\cdot g_i'(a)}\\
            &=\langle f'(a)^T,g(a)\rangle
            +\langle f(a),g'(a)^T\rangle.
        \end{align*}
    \end{solution}
    \part{
        If $f:\rl\to\ron$ is differentiable
        function and $\left\vert f(t)
        \right\vert=1$ for all $t$, show
        that $\langle f'(t)^T,f(t)
        \rangle = 0.$
    }
    \begin{solution}
        Define $h:\rl\to\rl$ by $h=\langle
        f(t),f(t)\rangle.$ Then
        $$h(t)=\lVert f(t)\rVert ^2=1$$
        From \ref{2-13, b}, we have
        $$h'(t)=2\langle f'(t)^T,f(t)
        \rangle.$$
        Since $h(t)=1,$ we have
        $ h'(t)=0$ and the
        required result follows.
    \end{solution}
    \part{
        Exhibit a differentiable function
        $f:\rl\to\rl$ such that the 
        function $\vert f\vert$ defined
        by $\vert f\vert(t)=\vert f(t)
        \vert$ is not differentiable.
    }
    \begin{solution}
        $f(t)=t$ is differentiable.
        $\vert f\vert(t)=
        \vert f(t)\vert=
        \vert t\vert$ is
        not differentiable.
    \end{solution}
\end{parts}