\question{
    [2-24] Define $f:\rl^2\to\rl$ by
    $$f(x,y)=\begin{dcases}
        xy\frac{x^2-y^2}{x^2+y^2}
        &(x,y)\ne 0,\\
        0&(x,y)=0.
    \end{dcases}$$
}
\begin{parts}
    \part{
        Show that $D_2f(x,0)=x$ for all
        $x$ and $D_1f(0,y)=-y$ for all
        y.
    }
    \begin{solution}
        Here,
        \begin{align*}
            D_2f(x,0)&=\lim_{h\to 0}{
                \frac{f(x,h)-f(x,0)}
                {h}
            }\\
            &=\lim_{h\to 0}{
            \frac{xh\dfrac{x^2-h^2
            }{x^2+h^2}-0}{h}}\\
            &=\lim_{h\to 0}{\dfrac
            {x(x^2-h^2)}{x^2+h^2}}\\
            &=x.
        \end{align*}
        Similarly, $D_2f(0,y)=-y$.
    \end{solution}

    \part{
        Show that $D_{1,2}f(0,0)
        \ne D_{2,1}
        f(0,0)$.
    }
    \begin{solution}
        We have,
        \begin{align*}
            D_{1,2}f(0,0)&=D_2(D_1)
            (f(0,0))\\
            &=\lim_{h\to 0}
            {\frac{D_1(0,h)-D_1(0,0)}
            {h}}\\
            &=\lim_{h\to 0}{\frac
            {-h}{h}}=-1.
        \end{align*}
        Similarly, we get $D_{2,1}
        f(0,0)=1$.
    \end{solution}
\end{parts}