\question{
    [2-29]
    Let $f:\ron\to\rl$. For $x\in\ron$,
    the limit
    $$\lim_{t\to 0}{\frac{f(a+tx)
    -f(a)}{t}},$$
    if it exists, is denoted $D_xf(a)$,
    and is called the 
    $\mathbf{directional}$
    derivarive of
    $f$ at $a$, in the direction $x$.
}

\begin{parts}
    \part{
        Show that $D_{e_i}f(a)=D_if(a)$.
    }
    \begin{solution}
        Here,
        \begin{align*}
        D_{e_i}f(a)&=\lim_{t\to 0}{
        \frac{f((a_1,...,a_i,...,a_n)+
        (0,...,t,...,0))-
        f(a_1,...,a_i,...,a_n)}{t}
        }\\
        &=\lim_{t\to 0}{
        \frac{f(a_1,...,a_i+t,...,a_n)-
        f(a_1,...,a_i,...,a_n)}{t}
        }=D_if(a).
        \end{align*}
    \end{solution}
    \part{
        Show that $D_{tx}f(a)=tD_xf(a)$.
    }
    \begin{solution}
        Since $th\to 0$ as $h\to 0$,
        for $t,h\in \rl$, we have
        $$D_{tx}f(a)=t\lim_{h\to 0}
        {\frac{f(a+thx)-f(a)}{th}}
        =tD_xf(a).$$
    \end{solution}

    \part{
        If $f$ is differentiable at $a$,
        show that $D_xf(a)=Df(a)(x)$, and
        therefore $D_{x+y}f(a)=D_xf(a)+
        D_yf(a)$.
    }
    \begin{solution}
        Here
        \begin{align*}
            Df(a)(x)
            &=\lVert x\rVert\lim_{x\to 0}
            {\dfrac{f(a+x)-f(a)}
            {\lVert x\rVert}}\\
            \shortintertext{and if
            $y\in\ron$, $ty\to 0$ as
            $t\to 0$. So for $y\neq 0$,}
            &=\lVert x\rVert\lim_{t\to 0}
            {\dfrac{f(a+ty)-f(a)}{\lVert ty
            \rVert}}\\
            &=\dfrac{\lVert x\rVert}
            {\lVert y\rVert}D_yf(a)\\
            &=t\cdot D_{x/t}f(a)=D_xf(a).
        \end{align*}
        Since $Df(a)$ is linear, the
        remaining results immediately follow.
    \end{solution}
\end{parts}